src/StorageScalarFamilyCompose.v
@@ -34,6 +34,54 @@ Arguments bssc_privatization_params {exp_value promo_value} _.
 Arguments bssc_promotion_params {exp_value promo_value} _.
 Arguments bssc_mid_program {exp_value promo_value} _.
 
+Definition scalar_storage_privatization_family
+    (exp_value: Type)
+    (exp_value_eqb: exp_value -> exp_value -> bool)
+    (exp_value_eqb_sound:
+      forall left right,
+        exp_value_eqb left right = true ->
+        left = right)
+    : View.checked_parameterized_view_transform_family
+        (Expansion.scalar_privatization_bounded_value_params exp_value) :=
+  Expansion.scalar_privatization_bounded_value_family
+    exp_value exp_value_eqb exp_value_eqb_sound.
+
+Definition scalar_storage_promotion_family
+    (promo_value: Type)
+    (promo_value_eqb: promo_value -> promo_value -> bool)
+    (promo_value_eqb_sound:
+      forall left right,
+        promo_value_eqb left right = true ->
+        left = right)
+    : View.checked_parameterized_view_transform_family
+        (Promotion.scalar_promotion_bounded_compatible_non_escape_value_params
+          promo_value) :=
+  Promotion.scalar_promotion_bounded_compatible_non_escape_value_family
+    promo_value promo_value_eqb promo_value_eqb_sound.
+
+Definition bounded_scalar_storage_pair_certificate
+    (exp_value promo_value: Type)
+    (exp_value_eqb: exp_value -> exp_value -> bool)
+    (promo_value_eqb: promo_value -> promo_value -> bool)
+    (exp_value_eqb_sound:
+      forall left right,
+        exp_value_eqb left right = true ->
+        left = right)
+    (promo_value_eqb_sound:
+      forall left right,
+        promo_value_eqb left right = true ->
+        left = right)
+    (certificate: bounded_scalar_storage_certificate exp_value promo_value)
+    : View.checked_parameterized_family_pair_certificate
+        (scalar_storage_privatization_family
+          exp_value exp_value_eqb exp_value_eqb_sound)
+        (scalar_storage_promotion_family
+          promo_value promo_value_eqb promo_value_eqb_sound) := {|
+  View.cpfpc_first_params := bssc_privatization_params certificate;
+  View.cpfpc_second_params := bssc_promotion_params certificate;
+  View.cpfpc_mid_program := bssc_mid_program certificate;
+|}.
+
 Definition bounded_scalar_storage_certificate_input_view
     {exp_value promo_value: Type}
     (certificate: bounded_scalar_storage_certificate exp_value promo_value)
@@ -68,33 +116,11 @@ Definition bounded_scalar_storage_certificate_accepted
         left = right)
     (certificate: bounded_scalar_storage_certificate exp_value promo_value)
     (before after: PolIRs.PolyLang.t) : Prop :=
-  exists privatization_ok promotion_ok,
-    mayReturn
-      (View.cpvtf_check
-        (Expansion.scalar_privatization_bounded_value_family
-          exp_value exp_value_eqb exp_value_eqb_sound)
-        (bssc_privatization_params certificate)
-        before (bssc_mid_program certificate))
-      privatization_ok /\
-    privatization_ok = true /\
-    View.cpvtf_side_condition
-      (Expansion.scalar_privatization_bounded_value_family
-        exp_value exp_value_eqb exp_value_eqb_sound)
-      (bssc_privatization_params certificate)
-      before (bssc_mid_program certificate) /\
-    mayReturn
-      (View.cpvtf_check
-        (Promotion.scalar_promotion_bounded_compatible_non_escape_value_family
-          promo_value promo_value_eqb promo_value_eqb_sound)
-        (bssc_promotion_params certificate)
-        (bssc_mid_program certificate) after)
-      promotion_ok /\
-    promotion_ok = true /\
-    View.cpvtf_side_condition
-      (Promotion.scalar_promotion_bounded_compatible_non_escape_value_family
-        promo_value promo_value_eqb promo_value_eqb_sound)
-      (bssc_promotion_params certificate)
-      (bssc_mid_program certificate) after.
+  View.checked_parameterized_family_pair_certificate_accepted
+    (bounded_scalar_storage_pair_certificate
+      exp_value promo_value exp_value_eqb promo_value_eqb
+      exp_value_eqb_sound promo_value_eqb_sound certificate)
+    before after.
 
 Theorem bounded_scalar_privatization_then_scalar_promotion_public_semantic_refinement :
   forall (exp_value promo_value: Type)
@@ -199,21 +225,18 @@ Proof.
   intros exp_value promo_value exp_value_eqb promo_value_eqb
          exp_value_eqb_sound promo_value_eqb_sound
          certificate before after Haccepted.
-  destruct Haccepted as [privatization_ok [promotion_ok Haccepted]].
-  destruct Haccepted as
-    [Hpriv_ret [Hpriv_ok [Hpriv_side
-     [Hpromotion_ret [Hpromotion_ok Hpromotion_side]]]]].
-  destruct certificate as
-    [privatization_params promotion_params mid].
-  simpl in *.
   exact
-    (bounded_scalar_privatization_then_scalar_promotion_public_semantic_refinement
-       exp_value promo_value exp_value_eqb promo_value_eqb
-       exp_value_eqb_sound promo_value_eqb_sound
-       privatization_params promotion_params
-       before mid after privatization_ok promotion_ok
-       Hpriv_ret Hpriv_ok Hpriv_side
-       Hpromotion_ret Hpromotion_ok Hpromotion_side).
+    (View.checked_parameterized_family_pair_certificate_public_semantic_sound
+       _
+       _
+       (scalar_storage_privatization_family
+          exp_value exp_value_eqb exp_value_eqb_sound)
+       (scalar_storage_promotion_family
+          promo_value promo_value_eqb promo_value_eqb_sound)
+       (bounded_scalar_storage_pair_certificate
+          exp_value promo_value exp_value_eqb promo_value_eqb
+          exp_value_eqb_sound promo_value_eqb_sound certificate)
+       before after Haccepted).
 Qed.
 
 Theorem accepted_bounded_scalar_storage_certificate_state_sound :
@@ -251,12 +274,19 @@ Proof.
          exp_value_eqb_sound promo_value_eqb_sound
          certificate before after st_target0 st_source0 st_target_after
          Haccepted Hinput Htarget.
-  eapply
-    (accepted_bounded_scalar_storage_certificate_public_semantic_refinement
-       exp_value promo_value exp_value_eqb promo_value_eqb
-       exp_value_eqb_sound promo_value_eqb_sound
-       certificate before after Haccepted);
-    eauto.
+  exact
+    (View.checked_parameterized_family_pair_certificate_state_sound
+       _
+       _
+       (scalar_storage_privatization_family
+          exp_value exp_value_eqb exp_value_eqb_sound)
+       (scalar_storage_promotion_family
+          promo_value promo_value_eqb promo_value_eqb_sound)
+       (bounded_scalar_storage_pair_certificate
+          exp_value promo_value exp_value_eqb promo_value_eqb
+          exp_value_eqb_sound promo_value_eqb_sound certificate)
+       before after st_target0 st_source0 st_target_after
+       Haccepted Hinput Htarget).
 Qed.
 
 End StorageScalarFamilyCompose.
